

la

Maths

$$a) x_n = \frac{\sqrt{9n^4+7} - (3n^2+7)}{\sqrt{9n^4+7} + (3n^2+7)} \cdot \frac{\sqrt{9n^4+7} + (3n^2+7)}{\sqrt{9n^4+7} + 3n^2+7}$$

$$x_n = \frac{9n^4+7 - 9n^4-7-6n^2}{\sqrt{9n^4+7} + 3n^2+7} = \frac{-6n^2}{\sqrt{\dots} + 3n^2+7}$$

$$= \frac{n^2(-6)}{n^2\sqrt{9+\frac{7}{n^4}} + n^2(3+\frac{7}{n^2})} = \frac{-6}{\sqrt{9+3} + 3} = \frac{-6}{6} = -1$$

\downarrow \downarrow
 0 0

$$b) x_n = (-1)^n \sqrt[n]{n^2 2^n} \rightarrow \left(n^{\frac{2}{n}}\right)^2$$

$$x_n = (-1)^n \cdot n^{\frac{2}{n}} \cdot 2$$

\uparrow
 $n \rightarrow \infty \rightarrow 1$

$\hookrightarrow (-1)^n \cdot 2 = \text{divergent (b)}$
 how $x_n(\text{even}) = 2$
 and $x_n(\text{odd}) = -2$

$$c) x_n = \frac{(p^{\frac{n-2}{n}} \cdot p^{\frac{2}{n}})^{n+1} \cdot q^{-n+1}}{q^{\frac{1}{n}} \cdot (q^{n-1})^{\frac{1}{n}} \cdot p^2} =$$

Simplification:

$$p^{\frac{n-2}{n}} \cdot p^{\frac{2}{n}} = p^{\frac{n-2}{n} + \frac{2}{n}} = p^{\frac{n-2+2}{n}} = p^{\frac{n}{n}} = p^1$$

$$\left(p^{\frac{n+1}{n}}\right)^{n+1} =$$

$$x_n = \frac{p^{n+1} \cdot q^{-n+1}}{q^{\frac{1}{n}} \cdot (q^{n-1})^{\frac{1}{n}} \cdot p^2} =$$

$$= \frac{p^{n+1} \cdot q^{-n+1}}{q^{\frac{1}{n}} p^2}$$

$$\hookrightarrow q^{\frac{1}{n}} \cdot q^{1-\frac{1}{n}} = q^{\frac{1}{n} + 1 - \frac{1}{n}} = q^1$$

$$\frac{p^{n+1} \cdot q^{-n+1}}{q p^2} = \frac{p^{n+1}}{p^2} \cdot \frac{q^{-n+1}}{q} =$$

$$p^{n-1} \cdot q^{-n} = \frac{p^{n-1}}{q^n} = \frac{p^{n-1}}{q^n} \rightarrow 0$$

$$p^n \cdot p^{-1} \cdot q^{-n} = \frac{1}{p} \cdot p^n \cdot q^{-n} =$$

$$\frac{1}{p} \left(\frac{p}{q}\right)^n \rightarrow 0 < p < q \Rightarrow 0 < \frac{p}{q} < 1$$

$$\lim_{n \rightarrow \infty} x_n = \left(\frac{p}{q}\right)^n \rightarrow 0$$

So limit is 0

Problem 2 Sequences

$$x_{n+1} = \sqrt{6 + x_n} \text{ for } n \in \mathbb{N}$$

$$x_2 = \sqrt{7}$$

$$x_3 = \sqrt{6 + \sqrt{7}}$$

$$(x_{n+1})^2 = (6 + x_n)$$

$$x_{n+1}^2 = 6 + x_n$$

$$x_{n+1}^2 - x_n - 6 = 0$$

$$x_n = L$$

$$L^2 - L - 6 = 0$$

$$L = -2 \leftarrow \text{impossible so } L = 3$$

$$L = 3$$

since $L=3$ is the limit

$\sqrt{6+x_n} \geq 0$ for all n because a square
so the sequence is bounded below
by 3. (a square root cannot be
negative)

Upper bound: Since the limit is 5
the sequence must be bounded above
by 5

Proof by induction (Monotonicity)

Base case

$$x_{n+1} = \sqrt{6+x_n} \quad x_2 = \sqrt{6+1} = \sqrt{7} > x_1$$

Inductive hypothesis, $n+1=k$

$$x_k = \sqrt{6+x_{k-1}}$$

$$x_{k+1} = \sqrt{6+x_k}$$

$$x_k \geq x_{k-1} \quad | +6$$

$$6+x_k \geq 6+x_{k-1} \quad | \sqrt{}$$

$$\sqrt{6+x_k} \geq \sqrt{6+x_{k-1}}$$

$$\begin{array}{c} \text{||} \\ x_{k+1} \end{array}$$

$$\begin{array}{c} \text{||} \\ x_k \end{array}$$

$$\text{So } x_{k+1} \geq x_k$$

Thus the sequence is ^{monotonically} bounded
increasing.